pico-ifc-coq/dyn_allocation/RefinementAC.v
@@ -38,11 +38,7 @@ Hypothesis stamp_cblock : Mem.stamp cblock = Kernel.
 
 Let ctable_impl : list CSysCallImpl := nil.
 
-Definition tini_fetch_rule_withsig :=
-  (fun opcode => existT _
-                        (QuasiAbstractMachine.labelCount opcode)
-                        (QuasiAbstractMachine.fetch_rule opcode)).
-Let faultHandler := FaultRoutine.faultHandler tini_fetch_rule_withsig.
+Let faultHandler := FaultRoutine.faultHandler _ QuasiAbstractMachine.fetch_rule.
 Let ctable := build_syscall_table (Z.of_nat (length faultHandler)) ctable_impl.
 
 Context {WFCLatt: WfConcreteLattice cblock ctable T Latt CLatt}.
@@ -58,7 +54,7 @@ Program Definition abstract_concrete_ref :
   refinement (abstract_machine atable) tini_concrete_machine :=
   @ref_composition _ _ _
                    (abstract_quasi_abstract_ref Hatable)
-                   (quasi_abstract_concrete_ref stamp_cblock atable fetch_rule)
+                   (quasi_abstract_concrete_ref stamp_cblock atable (fetch_rule:=fetch_rule))
                    (@ac_match_initial_data _ _ _ cblock fetch_rule)
                    match_events
                    _ _.
